fix more bigint warnings

concurrency/scache/Constants.i.dfy
@@ -3,15 +3,15 @@ include "../../lib/Lang/NativeTypes.s.dfy"
 module Constants {
   import opened NativeTypes
 
-  const RC_WIDTH := 24;
-  const CACHE_SIZE := 1048576;
-  const NUM_DISK_PAGES := 536870912;
+  const RC_WIDTH: uint64 := 24;
+  const CACHE_SIZE: uint64 := 1048576;
+  const NUM_DISK_PAGES: uint64 := 536870912;
 
-  const CHUNK_SIZE := 64;
-  const NUM_CHUNKS := CACHE_SIZE / 64;
-  const CLEAN_AHEAD := NUM_CHUNKS / 3;
+  const CHUNK_SIZE: uint64 := 64;
+  const NUM_CHUNKS: uint64 := CACHE_SIZE / 64;
+  const CLEAN_AHEAD: uint64 := NUM_CHUNKS / 3;
 
-  const NUM_IO_SLOTS := 128;
+  const NUM_IO_SLOTS: uint64 := 128;
 
   const DEFAULT_MAX_IO_EVENTS: uint64 := 32;
 }
