concurrency/scache/CacheInit.i.dfy
@@ -25,19 +25,19 @@ module CacheInit(aio: AIO(CacheAIOParams, CacheIfc, CacheSSM)) {
 
   glinear method split_into_page_size_chunks(glinear pta: PointsToArray<byte>)
   returns (glinear pta_seq: glseq<PointsToArray<byte>>)
-  requires |pta.s| == PageSize * CACHE_SIZE
-  ensures pta_seq.len() == CACHE_SIZE
-  ensures forall i {:trigger pta_seq.has(i)} | 0 <= i < CACHE_SIZE ::
+  requires |pta.s| == PageSize as int * CACHE_SIZE as int
+  ensures pta_seq.len() == CACHE_SIZE as int
+  ensures forall i {:trigger pta_seq.has(i)} | 0 <= i < CACHE_SIZE as int ::
       pta_seq.has(i)
-        && 0 <= pta.ptr.as_nat() + i * PageSize < 0x1_0000_0000_0000_0000
-        && pta_seq.get(i).ptr == ptr_add(pta.ptr, i as uint64 * PageSize as uint64)
-        && |pta_seq.get(i).s| == PageSize
+        && 0 <= pta.ptr.as_nat() + i * PageSize as int < 0x1_0000_0000_0000_0000
+        && pta_seq.get(i).ptr == ptr_add(pta.ptr, i as uint64 * PageSize)
+        && |pta_seq.get(i).s| == PageSize as int
 
   method init_batch_busy()
   returns (linear batch_busy: lseq<Atomic<bool, NullGhostType>>)
-  ensures |batch_busy| == NUM_CHUNKS
-  ensures (forall i :: 0 <= i < NUM_CHUNKS ==> lseq_has(batch_busy)[i])
-  ensures (forall i, v, g :: 0 <= i < NUM_CHUNKS ==> atomic_inv(batch_busy[i], v, g) <==> true)
+  ensures |batch_busy| == NUM_CHUNKS as int
+  ensures (forall i :: 0 <= i < NUM_CHUNKS as int ==> lseq_has(batch_busy)[i])
+  ensures (forall i, v, g :: 0 <= i < NUM_CHUNKS as int ==> atomic_inv(batch_busy[i], v, g) <==> true)
 
   method init_cache(glinear init_tok: T.Token)
   returns (linear c: Cache)
@@ -47,47 +47,47 @@ module CacheInit(aio: AIO(CacheAIOParams, CacheIfc, CacheSSM)) {
     var data_base_ptr;
     glinear var data_pta_full;
     data_base_ptr, data_pta_full := alloc_array_aligned<byte>(
-        CACHE_SIZE as uint64 * PageSize as uint64, 0, PageSize as uint64);
+        CACHE_SIZE * PageSize, 0, PageSize);
     glinear var data_pta_seq : glseq<PointsToArray<byte>> :=
         split_into_page_size_chunks(data_pta_full);
 
     var iocb_base_ptr;
     glinear var iocbs;
-    iocb_base_ptr, iocbs := new_iocb_array(NUM_IO_SLOTS as uint64);
+    iocb_base_ptr, iocbs := new_iocb_array(NUM_IO_SLOTS);
 
-    linear var read_refcounts_array := lseq_alloc<AtomicRefcount>(RC_WIDTH as uint64 * CACHE_SIZE as uint64);
-    linear var status_idx_array := lseq_alloc<StatusIdx>(CACHE_SIZE as uint64);
+    linear var read_refcounts_array := lseq_alloc<AtomicRefcount>(RC_WIDTH * CACHE_SIZE);
+    linear var status_idx_array := lseq_alloc<StatusIdx>(CACHE_SIZE);
 
     glinear var dis, empty_seq := split_init(init_tok);
 
-    ghost var data := seq(CACHE_SIZE, (i) requires 0 <= i < CACHE_SIZE =>
+    ghost var data := seq(CACHE_SIZE as int, (i) requires 0 <= i < CACHE_SIZE as int =>
         data_pta_seq.get(i).ptr);
 
     ghost var data_pta_seq_copy := data_pta_seq;
 
     var i: uint64 := 0;
-    while i < CACHE_SIZE as uint64
-    invariant 0 <= i as int <= CACHE_SIZE
-    invariant empty_seq == EmptySeq(i as nat, CACHE_SIZE)
-    invariant data_pta_seq.len() == CACHE_SIZE
-    invariant forall j | i as int <= j < CACHE_SIZE :: 
+    while i < CACHE_SIZE
+    invariant 0 <= i as int <= CACHE_SIZE as int
+    invariant empty_seq == EmptySeq(i as nat, CACHE_SIZE as int)
+    invariant data_pta_seq.len() == CACHE_SIZE as int
+    invariant forall j | i as int <= j < CACHE_SIZE as int :: 
         data_pta_seq.has(j) && data_pta_seq.get(j) == data_pta_seq_copy.get(j)
-    invariant |status_idx_array| == CACHE_SIZE
-    invariant forall j | i as int <= j < CACHE_SIZE :: j !in status_idx_array
+    invariant |status_idx_array| == CACHE_SIZE as int
+    invariant forall j | i as int <= j < CACHE_SIZE as int :: j !in status_idx_array
     invariant forall j | 0 <= j < i as int :: j in status_idx_array
         && status_idx_array[j].status.inv()
         && status_idx_array[j].status.key == Key(data[j], status_idx_array[j].idx, j)
 
-    invariant |read_refcounts_array| == RC_WIDTH * CACHE_SIZE
-    invariant forall i', j' | i as int <= i' < CACHE_SIZE && 0 <= j' < RC_WIDTH ::
-        (j' * CACHE_SIZE + i') !in read_refcounts_array
-    invariant forall i', j' | 0 <= i' < i as int && 0 <= j' < RC_WIDTH ::
-        (j' * CACHE_SIZE + i') in read_refcounts_array
-        && read_refcounts_array[j' * CACHE_SIZE + i'].inv(j')
-        && read_refcounts_array[j' * CACHE_SIZE + i'].rwlock_loc
+    invariant |read_refcounts_array| == RC_WIDTH as int * CACHE_SIZE as int
+    invariant forall i', j' | i as int <= i' < CACHE_SIZE as int && 0 <= j' < RC_WIDTH as int ::
+        (j' * CACHE_SIZE as int + i') !in read_refcounts_array
+    invariant forall i', j' | 0 <= i' < i as int && 0 <= j' < RC_WIDTH as int ::
+        (j' * CACHE_SIZE as int + i') in read_refcounts_array
+        && read_refcounts_array[j' * CACHE_SIZE as int + i'].inv(j')
+        && read_refcounts_array[j' * CACHE_SIZE as int + i'].rwlock_loc
             == status_idx_array[i'].status.rwlock_loc
 
-    decreases CACHE_SIZE - i as int
+    decreases CACHE_SIZE as int - i as int
     {
       linear var cell_idx;
       glinear var cell_idx_contents;
@@ -98,7 +98,7 @@ module CacheInit(aio: AIO(CacheAIOParams, CacheIfc, CacheSSM)) {
       ghost var key := Key(data_pta.ptr, cell_idx, i as nat);
 
       glinear var cache_empty;
-      cache_empty, empty_seq := pop_EmptySeq(empty_seq, i as nat, CACHE_SIZE);
+      cache_empty, empty_seq := pop_EmptySeq(empty_seq, i as nat, CACHE_SIZE as int);
       glinear var handle := CacheEmptyHandle(key, cache_empty, cell_idx_contents, data_pta);
       glinear var central, rcs := RwLockToken.perform_Init(handle);
       ghost var rwlock_loc := central.loc;
@@ -117,34 +117,34 @@ module CacheInit(aio: AIO(CacheAIOParams, CacheIfc, CacheSSM)) {
       lseq_give_inout(inout status_idx_array, i, status_idx);
 
       var j : uint64 := 0;
-      while j < RC_WIDTH as uint64
-      invariant 0 <= i as int < CACHE_SIZE
-      invariant 0 <= j as int <= RC_WIDTH
-      invariant rcs.val == RwLock.Rcs(j as nat, RC_WIDTH)
+      while j < RC_WIDTH
+      invariant 0 <= i as int < CACHE_SIZE as int
+      invariant 0 <= j as int <= RC_WIDTH as int
+      invariant rcs.val == RwLock.Rcs(j as nat, RC_WIDTH as int)
       invariant rcs.loc == rwlock_loc
 
-      invariant |read_refcounts_array| == RC_WIDTH * CACHE_SIZE
-      invariant forall i', j' | i as int < i' < CACHE_SIZE && 0 <= j' < RC_WIDTH ::
+      invariant |read_refcounts_array| == RC_WIDTH as int * CACHE_SIZE as int
+      invariant forall i', j' | i as int < i' < CACHE_SIZE as int && 0 <= j' < RC_WIDTH as int ::
           (j' * CACHE_SIZE as int + i') !in read_refcounts_array
-      invariant forall j' | j as int <= j' < RC_WIDTH ::
+      invariant forall j' | j as int <= j' < RC_WIDTH as int ::
           (j' * CACHE_SIZE as int + i as int) !in read_refcounts_array
       invariant forall i', j' |
-          (0 <= i' < i as int && 0 <= j' < RC_WIDTH) ::
-        (j' * CACHE_SIZE + i') in read_refcounts_array
-        && read_refcounts_array[j' * CACHE_SIZE + i'].inv(j')
-        && read_refcounts_array[j' * CACHE_SIZE + i'].rwlock_loc
+          (0 <= i' < i as int && 0 <= j' < RC_WIDTH as int) ::
+        (j' * CACHE_SIZE as int + i') in read_refcounts_array
+        && read_refcounts_array[j' * CACHE_SIZE as int + i'].inv(j')
+        && read_refcounts_array[j' * CACHE_SIZE as int + i'].rwlock_loc
             == status_idx_array[i'].status.rwlock_loc
       invariant forall j': int |
           (0 <= j' < j as int) ::
-        (j' * CACHE_SIZE + i as int) in read_refcounts_array
-        && read_refcounts_array[j' * CACHE_SIZE + i as int].inv(j')
-        && read_refcounts_array[j' * CACHE_SIZE + i as int].rwlock_loc
+        (j' * CACHE_SIZE as int + i as int) in read_refcounts_array
+        && read_refcounts_array[j' * CACHE_SIZE as int + i as int].inv(j')
+        && read_refcounts_array[j' * CACHE_SIZE as int + i as int].rwlock_loc
             == status_idx_array[i as int].status.rwlock_loc
 
-      decreases RC_WIDTH - j as int
+      decreases RC_WIDTH as int - j as int
       {
         glinear var rc;
-        rc, rcs := RwLockToken.pop_rcs(rcs, j as nat, RC_WIDTH);
+        rc, rcs := RwLockToken.pop_rcs(rcs, j as nat, RC_WIDTH as int);
         linear var ar_atomic := new_atomic(0, rc,
             (v, g) => AtomicRefcountImpl.state_inv(v, g, j as nat, rwlock_loc),
             0);
@@ -152,7 +152,7 @@ module CacheInit(aio: AIO(CacheAIOParams, CacheIfc, CacheSSM)) {
 
         // XXX I don't care about the perf of the initialization method, but do note
         // that the access pattern for writing to this array might be completely awful.
-        lseq_give_inout(inout read_refcounts_array, j * CACHE_SIZE as uint64 + i, ar);
+        lseq_give_inout(inout read_refcounts_array, j * CACHE_SIZE + i, ar);
 
         j := j + 1;
       }
@@ -164,20 +164,20 @@ module CacheInit(aio: AIO(CacheAIOParams, CacheIfc, CacheSSM)) {
 
     assert {:split_here} true;
 
-    linear var cache_idx_of_page_array := lseq_alloc(NUM_DISK_PAGES as uint64);
+    linear var cache_idx_of_page_array := lseq_alloc(NUM_DISK_PAGES);
 
     var i2 := 0;
-    while i2 < NUM_DISK_PAGES as uint64
-    invariant 0 <= i2 as int <= NUM_DISK_PAGES
-    invariant dis == IdxsSeq(i2 as nat, NUM_DISK_PAGES);
-    invariant |cache_idx_of_page_array| == NUM_DISK_PAGES
-    invariant forall j | i2 as int <= j < NUM_DISK_PAGES :: j !in cache_idx_of_page_array
+    while i2 < NUM_DISK_PAGES
+    invariant 0 <= i2 as int <= NUM_DISK_PAGES as int
+    invariant dis == IdxsSeq(i2 as nat, NUM_DISK_PAGES as int);
+    invariant |cache_idx_of_page_array| == NUM_DISK_PAGES as int
+    invariant forall j | i2 as int <= j < NUM_DISK_PAGES as int :: j !in cache_idx_of_page_array
     invariant forall j | 0 <= j < i2 as int :: j in cache_idx_of_page_array
         && atomic_index_lookup_inv(cache_idx_of_page_array[j], j)
-    decreases NUM_DISK_PAGES - i2 as int
+    decreases NUM_DISK_PAGES as int - i2 as int
     {
       glinear var di;
-      di, dis := pop_IdxSeq(dis, i2 as nat, NUM_DISK_PAGES);
+      di, dis := pop_IdxSeq(dis, i2 as nat, NUM_DISK_PAGES as int);
       linear var ail := new_atomic(NOT_MAPPED, di,
           (v, g) => AtomicIndexLookupImpl.state_inv(v, g, i2 as nat),
           0);
@@ -190,20 +190,20 @@ module CacheInit(aio: AIO(CacheAIOParams, CacheIfc, CacheSSM)) {
     dispose_anything(dis);
 
     linear var global_clockpointer := new_atomic(0, NullGhostType, (v, g) => true, 0);
-    linear var io_slots := lseq_alloc<IOSlot>(NUM_IO_SLOTS as uint64);
+    linear var io_slots := lseq_alloc<IOSlot>(NUM_IO_SLOTS);
 
     ghost var iocbs_copy := iocbs;
 
     assert {:split_here} true;
 
-    var i3 := 0;
-    while i3 < NUM_IO_SLOTS as uint64
-    invariant 0 <= i3 as int <= NUM_IO_SLOTS
-    invariant iocbs.len() == NUM_IO_SLOTS
-    invariant forall j | i3 as int <= j < NUM_IO_SLOTS :: 
+    var i3: uint64 := 0;
+    while i3 < NUM_IO_SLOTS
+    invariant 0 <= i3 as int <= NUM_IO_SLOTS as int
+    invariant iocbs.len() == NUM_IO_SLOTS as int
+    invariant forall j | i3 as int <= j < NUM_IO_SLOTS as int ::
         iocbs.has(j) && iocbs.get(j) == iocbs_copy.get(j)
-    invariant |io_slots| == NUM_IO_SLOTS
-    invariant forall j | i3 as int <= j < NUM_IO_SLOTS :: j !in io_slots
+    invariant |io_slots| == NUM_IO_SLOTS as int
+    invariant forall j | i3 as int <= j < NUM_IO_SLOTS as int :: j !in io_slots
     invariant forall j | 0 <= j < i3 as int :: j in io_slots
         && io_slots[j].WF()
         && iocb_base_ptr.as_nat() + j * SizeOfIocb() as int < 0x1_0000_0000_0000_0000
@@ -236,16 +236,16 @@ module CacheInit(aio: AIO(CacheAIOParams, CacheIfc, CacheSSM)) {
 
     assert {:split_here} true;
 
-    ghost var disk_idx_of_entry := seq(CACHE_SIZE, (i) requires 0 <= i < CACHE_SIZE =>
+    ghost var disk_idx_of_entry := seq(CACHE_SIZE as int, (i) requires 0 <= i < CACHE_SIZE as int =>
         status_idx_array[i].idx);
-    ghost var status := seq(CACHE_SIZE, (i) requires 0 <= i < CACHE_SIZE =>
+    ghost var status := seq(CACHE_SIZE as int, (i) requires 0 <= i < CACHE_SIZE as int =>
         status_idx_array[i].status);
     ghost var read_refcounts :=
-        seq(RC_WIDTH, (j) requires 0 <= j < RC_WIDTH =>
-          seq(CACHE_SIZE, (i) requires 0 <= i < CACHE_SIZE =>
-            read_refcounts_array[j * CACHE_SIZE + i]));
+        seq(RC_WIDTH as int, (j) requires 0 <= j < RC_WIDTH as int =>
+          seq(CACHE_SIZE as int, (i) requires 0 <= i < CACHE_SIZE as int =>
+            read_refcounts_array[j * CACHE_SIZE as int + i]));
     ghost var cache_idx_of_page :=
-        seq(NUM_DISK_PAGES, (i) requires 0 <= i < NUM_DISK_PAGES =>
+        seq(NUM_DISK_PAGES as int, (i) requires 0 <= i < NUM_DISK_PAGES as int =>
           cache_idx_of_page_array[i]);
 
     linear var ioctx := aio.init_ctx(
@@ -274,31 +274,31 @@ module CacheInit(aio: AIO(CacheAIOParams, CacheIfc, CacheSSM)) {
         io_slots,
         ioctx);
 
-    forall i | 0 <= i < CACHE_SIZE
-    ensures data[i].aligned(PageSize)
+    forall i | 0 <= i < CACHE_SIZE as int
+    ensures data[i].aligned(PageSize as int)
     {
     }
 
-    forall j, i | 0 <= j < RC_WIDTH && 0 <= i < CACHE_SIZE
+    forall j, i | 0 <= j < RC_WIDTH as int && 0 <= i < CACHE_SIZE as int
     ensures read_refcounts[j][i].inv(j)
     ensures read_refcounts[j][i].rwlock_loc == status[i].rwlock_loc
     {
       assert read_refcounts[j][i] == 
-          read_refcounts_array[j * CACHE_SIZE + i];
-      assert read_refcounts_array[j * CACHE_SIZE + i].inv(j);
+          read_refcounts_array[j * CACHE_SIZE as int + i];
+      assert read_refcounts_array[j * CACHE_SIZE as int + i].inv(j);
     }
 
-    var i0 := CACHE_SIZE - 1;
+    var i0 := CACHE_SIZE as int - 1;
     assert data_pta_seq_copy.has(i0);
-    assert 0 <= data_pta_full.ptr.as_nat() + i0 * PageSize < 0x1_0000_0000_0000_0000;
+    assert 0 <= data_pta_full.ptr.as_nat() + i0 * PageSize as int < 0x1_0000_0000_0000_0000;
 
-    forall i | 0 <= i < RC_WIDTH * CACHE_SIZE
+    forall i | 0 <= i < RC_WIDTH as int * CACHE_SIZE as int
     ensures lseq_has(read_refcounts_array)[i]
     {
-      var i1 := i % CACHE_SIZE;
-      var j1 := i / CACHE_SIZE;
-      assert i == j1 * CACHE_SIZE + i1;
-      assert lseq_has(read_refcounts_array)[j1 * CACHE_SIZE + i1];
+      var i1 := i % CACHE_SIZE as int;
+      var j1 := i / CACHE_SIZE as int;
+      assert i == j1 * CACHE_SIZE as int + i1;
+      assert lseq_has(read_refcounts_array)[j1 * CACHE_SIZE as int + i1];
     }
 
     assert c.Inv();
